Finish last lemma Normalization (substition_all) Show that there exists an instantiation for R

2016/Normalization.thy
@@ -2,10 +2,11 @@ theory Normalization
 imports 
   Main
   "~~/src/HOL/IMP/Star"
+  "$AFP/List-Index/List_Index"
 begin
 
 datatype ltype=
-  A | Fun ltype ltype ("_\<rightarrow>_" [100,100] 225)
+  A | Fun ltype ltype (infixr "\<rightarrow>"  225)
 
 datatype lterm=
   LVar nat | LApp lterm lterm | LAbs ltype lterm | ValA
@@ -42,6 +43,8 @@ inductive eval1_L :: "lterm \<Rightarrow> lterm \<Rightarrow> bool" where
     "is_value_L v2 \<Longrightarrow> eval1_L (LApp (LAbs T' t12) v2)
       (shift_L (-1) 0 (subst_L 0 (shift_L 1 0 v2) t12))" 
 
+inductive_cases eval1_LAppE: "eval1_L (LApp t1 t2) t'"
+
 type_synonym lcontext = "ltype list"
 
 
@@ -67,7 +70,12 @@ inductive has_type_L :: "lcontext \<Rightarrow> lterm \<Rightarrow> ltype \<Righ
   has_type_LAbs:
     "(\<Gamma> |,| T1) \<turnstile> t2 |:| T2 \<Longrightarrow> \<Gamma> \<turnstile> LAbs T1 t2 |:| (T1 \<rightarrow> T2)" |
   has_type_LApp:
-    "\<Gamma> \<turnstile> t1 |:| (T11 \<rightarrow> T12) \<Longrightarrow> \<Gamma> \<turnstile> t2 |:| T11 \<Longrightarrow> \<Gamma> \<turnstile> LApp t1 t2 |:| T12"
+    "\<Gamma> \<turnstile> t1 |:| T11 \<rightarrow> T12 \<Longrightarrow> \<Gamma> \<turnstile> t2 |:| T11 \<Longrightarrow> \<Gamma> \<turnstile> LApp t1 t2 |:| T12"
+
+lemma canonical_forms:
+  "is_value_L v \<Longrightarrow> \<Gamma> \<turnstile> v |:| A \<Longrightarrow> v = ValA"
+  "is_value_L v \<Longrightarrow> \<Gamma> \<turnstile> v |:| T1 \<rightarrow> T2 \<Longrightarrow> \<exists>t. v = LAbs T1 t"
+by (auto elim: has_type_L.cases is_value_L.cases)
 
 abbreviation closed ::"lterm \<Rightarrow> bool" where
   "closed t \<equiv> FV t={}"
@@ -79,12 +87,32 @@ locale rel_reasoning =
   fixes R::"lterm \<Rightarrow> ltype \<Rightarrow> bool" ("(_)\<in>\<^sub>R(_)" [150,150] 200)
   assumes R\<^sub>A: " halts t = t \<in>\<^sub>R A" and 
           R_fun: " (halts t \<and>
-            (\<forall>s. s \<in>\<^sub>R T1 \<longrightarrow> (LApp t s) \<in>\<^sub>R T2)) = t \<in>\<^sub>R (T1\<rightarrow>T2)" and
+            (\<forall>s. s \<in>\<^sub>R T1 \<longrightarrow> (LApp t s) \<in>\<^sub>R T2)) = t \<in>\<^sub>R T1\<rightarrow>T2" and
           R_def: "t\<in>\<^sub>RT \<Longrightarrow> closed t \<and> \<emptyset> \<turnstile> t |:| T"
 
 lemma (in rel_reasoning) R_halts:
   "t \<in>\<^sub>R T \<Longrightarrow> halts t"
 by (induction T, insert R\<^sub>A[of t] R_fun[of t], auto)
+
+lemma value_characterisation:
+  "\<Gamma> \<turnstile> t |:| T \<Longrightarrow> \<Gamma> = \<emptyset> \<Longrightarrow> \<forall>t1. \<not> eval1_L t t1 \<Longrightarrow> is_value_L t"
+proof (induction rule:"has_type_L.induct")
+  case (has_type_LApp \<Gamma> t1 T1 T2 t2)
+    have "\<exists>t. eval1_L (LApp t1 t2) t"
+      proof (cases "\<exists>t1'. eval1_L t1 t1'")
+        case (True)
+          thus ?thesis
+            by (auto intro: eval1_LApp1)
+      next
+        case (False)
+          thus ?thesis
+            using has_type_LApp(3)[OF has_type_LApp(5)]
+                  has_type_LApp(4)[OF has_type_LApp(5)]
+                  canonical_forms(2)[OF _ has_type_LApp(1)]
+            by (cases "\<exists>t2'. eval1_L t2 t2'", auto intro: eval1_L.intros) 
+      qed
+    with has_type_LApp(6) show ?case by blast
+qed (auto intro: "is_value_L.intros")
 
 lemma[simp]: "nat (int x + 1) = Suc x" by simp
 lemma[simp]: "nat (1 + int x) = Suc x" by simp
@@ -109,11 +137,65 @@ proof (induction u arbitrary: n t rule: lterm.induct)
         (metis DiffI One_nat_def UnCI diff_Suc_1 empty_iff imageI insert_iff nat.distinct(1))+)
 qed (auto simp: gr0_conv_Suc image_iff FV_shift[of 1, unfolded int_1])
 
-lemma eval_det:
-  "eval1_L t t1 \<Longrightarrow> eval1_L t t2 \<Longrightarrow> t1=t2" sorry
+theorem eval_det:
+  "eval1_L t t1 \<Longrightarrow> eval1_L t t2 \<Longrightarrow> t1=t2"
+proof (induction t t1 arbitrary: t2 rule: eval1_L.induct)
+  case (eval1_LApp1 t1 t1' t2)
+    from eval1_LApp1.hyps eval1_LApp1.prems show ?case
+      by (auto elim: eval1_L.cases is_value_L.cases intro: eval1_LApp1.IH)
+next
+  case (eval1_LApp2 t1 t2 t2')
+    from eval1_LApp2.hyps eval1_LApp2.prems show ?case
+      by (auto elim: eval1_L.cases is_value_L.cases intro: eval1_LApp2.IH)
+next
+  case (eval1_LApp_LAbs v2 t12)
+    thus ?case by (auto elim: eval1_L.cases simp: is_value_L.simps)
+qed
 
-lemma preservation:
-  "\<Gamma>\<turnstile> t|:| T \<Longrightarrow> eval1_L t t' \<Longrightarrow> \<Gamma> \<turnstile> t'|:| T" sorry
+lemma weakening:
+  "\<Gamma> \<turnstile> t |:| T \<Longrightarrow> n \<le> length \<Gamma> \<Longrightarrow> insert_nth n S \<Gamma> \<turnstile> shift_L 1 n t |:| T"
+proof (induction \<Gamma> t T arbitrary: n rule: has_type_L.induct)
+  case (has_type_LAbs \<Gamma> T1 t2 T2)
+    from has_type_LAbs.prems has_type_LAbs.hyps
+      has_type_LAbs.IH[where n="Suc n"] 
+    show ?case
+      by (auto intro: has_type_L.intros)
+qed (auto simp: nth_append min_def intro: has_type_L.intros)
+
+lemma substitution:
+  "\<Gamma> \<turnstile> t |:| T \<Longrightarrow>  \<Gamma> \<turnstile> LVar n |:| S \<Longrightarrow> \<Gamma> \<turnstile> s |:| S \<Longrightarrow> \<Gamma> \<turnstile> subst_L n s t |:| T"
+proof (induction \<Gamma> t T arbitrary: s n rule: has_type_L.induct)
+  case (has_type_LAbs \<Gamma> T1 t T2)
+  thus ?case by (fastforce
+    intro: has_type_L.intros weakening[where n=0, unfolded insert_nth_def nat.rec]
+    simp: has_type_L.simps[of _ "LVar n" _, simplified])
+qed (auto intro!: has_type_L.intros 
+          simp: has_type_L.simps[of _ "LVar _" _, simplified])
+
+lemma shift_down:
+  "insert_nth n U \<Gamma> \<turnstile> t |:| T \<Longrightarrow> n \<le> length \<Gamma> \<Longrightarrow>
+   (\<And>x. x \<in> FV t \<Longrightarrow> x \<noteq> n) \<Longrightarrow> \<Gamma> \<turnstile> shift_L (- 1) n t |:| T"
+proof (induction "insert_nth n U \<Gamma>" t T arbitrary: \<Gamma> n rule: has_type_L.induct)
+  case (has_type_LAbs V t T)
+  from this(1,3,4) show ?case
+    by (fastforce intro: has_type_L.intros has_type_LAbs.hyps(2)[where n="Suc n"])+
+qed (fastforce intro: has_type_L.intros simp: nth_append min_def)+
+
+
+theorem preservation:
+  "\<Gamma>\<turnstile> t|:| T \<Longrightarrow> eval1_L t t' \<Longrightarrow> \<Gamma> \<turnstile> t'|:| T" 
+proof (induction \<Gamma> t T arbitrary: t' rule: has_type_L.induct)
+  case (has_type_LApp \<Gamma> t1 T11 T12 t2)
+    note hyps = this and has_T_Abs= has_type_L.simps[of _ "LAbs _ _", simplified]
+         
+    from hyps show ?case  by (auto
+      intro!: has_type_L.intros substitution shift_down
+      dest: weakening[where n=0, unfolded insert_nth_def nat.rec]
+      elim!: eval1_LAppE
+      split: lterm.splits if_splits
+      simp: FV_subst FV_shift[of 1, unfolded int_1] has_T_Abs) 
+        (metis neq0_conv)
+qed (auto elim: eval1_L.cases)
 
 
 lemma halting_evalL:
@@ -138,6 +220,9 @@ next
       by metis
 qed
 
+lemma shift_shift_invert: "a>0 \<Longrightarrow> shift_L (-a) b (shift_L a b t) = t"
+by (induction t arbitrary: a b, auto)
+
 lemma halting_evalR:
   "eval1_L t t1 \<Longrightarrow> halts t1 \<Longrightarrow> halts t"
 by (induction rule: eval1_L.induct) (metis eval1_L.intros star_trans star_step1)+
@@ -146,6 +231,26 @@ theorem halting_eval:
   "eval1_L t t1 \<Longrightarrow> halts t = halts t1"
 using halting_evalL halting_evalR by blast
 
+lemma preservation_step:
+  "star eval1_L t t' \<Longrightarrow> \<Gamma> \<turnstile> t |:| T \<Longrightarrow> \<Gamma> \<turnstile> t' |:| T"
+by (induction rule: star.induct, auto intro: preservation)
+
+lemma (in rel_reasoning)halt_val:
+  "t \<in>\<^sub>R T \<Longrightarrow>\<exists>v. is_value_L v \<and> star eval1_L t v"
+proof -
+  assume Rt: "t \<in>\<^sub>R T"
+ 
+  have 1: "\<And>t'. star eval1_L t t' \<Longrightarrow> \<forall>t1. \<not> eval1_L t' t1 \<Longrightarrow> \<exists>v. is_value_L v \<and> star eval1_L t v"
+    using value_characterisation[of \<emptyset> _ T]
+          preservation_step[OF _ R_def[OF Rt, THEN conjunct2]]
+    by auto      
+  have "\<forall>t1.\<not> eval1_L t t1 \<Longrightarrow> \<exists>v. is_value_L v \<and> star eval1_L t v"
+    using value_characterisation[OF R_def[OF Rt, THEN conjunct2]]
+          star.refl[of "eval1_L"]
+    by auto
+
+  with 1 show "\<exists>v. is_value_L v \<and> star eval1_L t v" using R_halts[OF Rt] by auto
+qed  
 
 lemma (in rel_reasoning) eval_preserves_R:
   "\<Gamma> \<turnstile> t|:|T \<Longrightarrow> eval1_L t t' \<Longrightarrow> t \<in>\<^sub>R T \<Longrightarrow> t'\<in>\<^sub>R T"
@@ -170,13 +275,163 @@ next
       by auto
 qed
 
-abbreviation subst_all:: "lterm list \<Rightarrow> lterm \<Rightarrow> lterm" where
-"subst_all V \<equiv> rec_nat id (\<lambda>i r. r \<circ> (subst_L i (V!i))) (length V)"
+lemma (in rel_reasoning) eval_preserves_R2:
+  "\<Gamma> \<turnstile> t|:|T \<Longrightarrow> eval1_L t t' \<Longrightarrow> t' \<in>\<^sub>R T \<Longrightarrow> t\<in>\<^sub>R T"
+proof (induction T arbitrary: \<Gamma> t t')
+  case (A)
+    show ?case 
+      using A(3)[unfolded R\<^sub>A[symmetric] halting_eval[OF A(2), symmetric]]
+            R\<^sub>A[of t]
+      by auto
+next
+  case (Fun T1 T2)
+    note hyps=this
+    have "(\<forall>s. s\<in>\<^sub>RT1 \<longrightarrow> LApp t s\<in>\<^sub>RT2)" 
+      using hyps(2)[of \<emptyset>, OF _ eval1_LApp1[OF hyps(4)]]
+            hyps(5)[unfolded R_fun[symmetric], THEN conjunct2]
+            R_def[of "LApp t' _" T2] 
+      sorry
+    then show ?case
+      using R_fun[of t T1 T2]
+            hyps(5)[unfolded R_fun[symmetric] halting_eval[OF hyps(4),symmetric]]
+      by auto
+qed
+
+fun subst_all :: "nat \<Rightarrow> lterm list \<Rightarrow> lterm \<Rightarrow> lterm" where
+  "subst_all n V ValA = ValA" |
+  "subst_all n V (LApp s t) = LApp (subst_all n V s) (subst_all n V t)"|
+  "subst_all n V (LAbs T t) = LAbs T (subst_all (Suc n) (map (shift_L 1 0) V) t)"|
+  "subst_all n V (LVar k) = (if (k\<ge>n \<and> (k-n)<length V) then (V!(k-n)) else LVar k)"
+
+lemma subst_all_empty[simp]:
+  "subst_all n [] t = t"
+by (induction t arbitrary: n, auto)
+
+lemma subst_free_var_only: "x\<notin>FV t \<Longrightarrow> subst_L x t1 t = t"
+by (induction t arbitrary:t1 x, force+)
+
+lemma subst_all_shift:
+  "shift_L d c (subst_all n V t) = subst_all n (map (shift_L d c) V) t"
+sorry
+
+lemma subst_comp_subst_all:
+  "subst_L n v (subst_all (Suc n) (map (shift_L ((int n) + 1) 0) V) t) = subst_all n (v#map (shift_L ((int n) + 1) 0) V) t"
+proof (induction t arbitrary: n v)
+  case (LVar k)
+    have H:"\<And>s. n \<notin> FV (shift_L ((int n) + 1) 0 s)" 
+      proof (rule)
+        fix s
+       
+        assume H:"n \<in> FV (shift_L ((int n) + 1) 0 s)"
+        have H1:"1+int n = int n +1" by auto
+
+        show "False"
+          using FV_shift[of "n+1" 0 s, simplified]
+                image_iff[of n "\<lambda>x. Suc (x + n)" "FV s"]
+                H[unfolded H1[symmetric]]
+          by force
+      qed    
+          
+    from LVar show ?case
+      using subst_free_var_only[OF H]
+      by auto
+next
+  case (LAbs T t)
+    have H:"\<And>k. shift_L 1 k \<circ> shift_L (int n + 1) k= shift_L (int (Suc n) + 1) k"
+      proof 
+        fix k s 
+        show "(shift_L 1 k \<circ> shift_L (int n + 1) k) s= shift_L (int (Suc n) + 1) k s"
+          by (induction s arbitrary:k, auto)
+      qed
+    then show ?case using LAbs[of "Suc n"] by simp
+qed auto
 
 lemma (in rel_reasoning) subst_R:
-  "\<Gamma> \<turnstile> t |:| T \<Longrightarrow> length V = length \<Gamma> \<Longrightarrow> (\<And>i. i<length V \<Longrightarrow> (V!i) \<in>\<^sub>R (\<Gamma>!i)) \<Longrightarrow> 
-    subst_all V t \<in>\<^sub>R T"
-sorry
+  "\<Gamma> \<turnstile> t |:| T \<Longrightarrow> length V = length \<Gamma> \<Longrightarrow> (\<And>i. i<length V \<Longrightarrow>is_value_L (V!i) \<and> (V!i) \<in>\<^sub>R (\<Gamma>!i)) \<Longrightarrow> 
+    subst_all 0 V t \<in>\<^sub>R T"
+proof (induction arbitrary: V rule:has_type_L.induct)
+  case (has_type_LVar x T \<Gamma>)
+    have "V\<noteq>\<emptyset> \<Longrightarrow> \<exists>v V'. V= v#V'"
+      by (meson list.exhaust)
+    with has_type_LVar show ?case
+      by(cases "V=\<emptyset>", auto)      
+next
+  case (has_type_LApp \<Gamma> t1 T1 T2 t2)
+    note hyps=this
+    show ?case
+      using hyps(3)[OF hyps(5,6), unfolded R_fun[symmetric], simplified,
+                    THEN conjunct2]
+            hyps(4)[OF hyps(5,6),simplified]
+      by auto
+next
+  case (has_type_LAbs \<Gamma> T1 t T2)
+    note hyps=this
+    have "\<And>s. s\<in>\<^sub>RT1 \<Longrightarrow> LApp (LAbs T1 (subst_all (Suc 0) (map (shift_L 1 0) V) t)) s\<in>\<^sub>RT2"
+      proof -
+        fix s
+        assume Rs: "s \<in>\<^sub>R T1"
+        obtain v where v_prop:"is_value_L v" "star eval1_L s v"
+          using halt_val[OF Rs]
+          by auto
+        from this(2) have Rv:"v \<in>\<^sub>R T1"
+          using Rs
+          proof (induction rule:star.induct)
+            case (step x y z)
+              thus ?case using eval_preserves_R R_def
+                by force
+          qed force
+        have "shift_L (-1) 0 \<circ> shift_L 1 0 = id"
+          proof
+            fix x
+            show "(shift_L (-1) 0 \<circ> shift_L 1 0) x = id x"
+              using shift_shift_invert[of 1, simplified]
+              by auto
+          qed
+        hence ev1:"star eval1_L (LApp (LAbs T1 (subst_all (Suc 0) (map (shift_L 1 0) V) t)) v) 
+                             (subst_all 0 (v # V) t)"
+          using eval1_LApp_LAbs[OF v_prop(1),of T1 "subst_all (Suc 0) (map (shift_L 1 0) V) t"]
+                subst_comp_subst_all[of 0 "shift_L 1 0 v" V t, simplified]
+                subst_all_shift[of "-1" 0 0 _ t]
+                shift_shift_invert[of 1, simplified]
+          by force
+        have "star eval1_L (LApp (LAbs T1 (subst_all (Suc 0) (map (shift_L 1 0) V) t)) s)
+                (LApp (LAbs T1 (subst_all (Suc 0) (map (shift_L 1 0) V) t)) v)"
+          using v_prop(2,1)
+          proof (induction rule: star.induct)
+            case (step x y z)
+              show ?case
+                using star.intros(2)[OF _ step(3)[OF step(4)]]
+                      "is_value_L.intros"(2) eval1_LApp2[OF _ step(1)] 
+                by blast                      
+          qed auto
+        with ev1 have eval:"star eval1_L (LApp (LAbs T1 (subst_all (Suc 0) (map (shift_L 1 0) V) t)) s)
+                            (subst_all 0 (v # V) t)"
+          using star_trans[of "eval1_L"]
+          by meson
+        have type: "\<emptyset> \<turnstile> LApp (LAbs T1 (subst_all (Suc 0) (map (shift_L 1 0) V) t)) v |:| T2"
+          using R_def[of "subst_all 0 (v # V) t" T2]
+                substitution[OF hyps(1), of _ "(\<Gamma>|,|T1)!_" "shift_L 1 0 (V!_)"] hyps(4)
+                weakening[of \<emptyset> "V!_" "\<Gamma>!_" 0 T1, simplified]
+                R_def[OF Rv, THEN conjunct2]
+                has_type_L.intros(3,4)
+          sorry
+        thm hyps(2)[of "v#V",simplified]
+        show "LApp (LAbs T1 (subst_all (Suc 0) (map (shift_L 1 0) V) t)) s\<in>\<^sub>RT2"
+          using v_prop(1) 
+                R_def[OF Rs, THEN conjunct2] value_characterisation
+                hyps(2)[of "v# V", simplified]
+                eval_preserves_R2
+                eval
+                
+                
+                
+          sorry
+      qed
+    then show ?case
+      using R_fun[symmetric]
+            eval1_L.simps[of "LAbs T1 _", simplified]
+      by auto     
+qed (insert R\<^sub>A, auto intro!: has_type_L.intros eval1_L.simps[of ValA, simplified])
 
 theorem (in rel_reasoning) Normalization:
   "\<emptyset>\<turnstile> t |:| T \<Longrightarrow> halts t"
